\begin{enumerate}
\item $ \rightarrow   \exists  x (( \forall  z P(z))  \vee  !P(x))$\\
 from [2] by rule $\exists \rightarrow $ with new term $\alpha$
\item $ \rightarrow  ( \forall  z P(z))  \vee  !P(\alpha),  \exists  x (( \forall  z P(z))  \vee  !P(x))$\\
 from [3] by rule $ \vee \rightarrow $
\item $ \rightarrow  !P(\alpha),  \forall  z P(z),  \exists  x (( \forall  z P(z))  \vee  !P(x))$\\
 from [4] by rule $NOT\rightarrow $
\item $P(\alpha) \rightarrow   \forall  z P(z),  \exists  x (( \forall  z P(z))  \vee  !P(x))$\\
 from [5] by rule $\forall \rightarrow $ with new term $w1$
\item $P(\alpha) \rightarrow  P(w1),  \exists  x (( \forall  z P(z))  \vee  !P(x))$\\
 from [6] by rule $\exists \rightarrow $ with new term $\beta$
\item $P(\alpha) \rightarrow  P(w1), ( \forall  z P(z))  \vee  !P(\beta),  \exists  x (( \forall  z P(z))  \vee  !P(x))$\\
  used in temporary unifications: [4]\\
 from [7] by rule $ \vee \rightarrow $
\item $P(\alpha) \rightarrow  P(w1), !P(\beta),  \forall  z P(z),  \exists  x (( \forall  z P(z))  \vee  !P(x))$\\
 from [8] by rule $NOT\rightarrow $
\item $P(\beta), P(\alpha) \rightarrow  P(w1),  \forall  z P(z),  \exists  x (( \forall  z P(z))  \vee  !P(x))$\\
 from [9] by rule $\forall \rightarrow $ with new term $w2$
\item $P(\alpha), P(\beta) \rightarrow  P(w2), P(w1),  \exists  x (( \forall  z P(z))  \vee  !P(x))$\\ 
 unification succeded using [$\beta \mapsto w1$]
\end{enumerate}
