%\documentclass{cw1}
%\begin{document}

\begin{enumerate}
\item $ \rightarrow   \exists  x ( \exists  y (P(x)  \Rightarrow  ( \forall  x ( \forall  y P(y)))))$\\
 from [2] by rule $\exists \rightarrow $ with new term $\alpha$
\item $ \rightarrow   \exists  x ( \exists  y (P(x)  \Rightarrow  ( \forall  x ( \forall  y P(y))))),  \exists  y (P(\alpha)  \Rightarrow  ( \forall  x ( \forall  y P(y))))$\\
 from [3] by rule $\exists \rightarrow $ with new term $\beta$
\item $ \rightarrow  P(\alpha)  \Rightarrow  ( \forall  x ( \forall  y P(y))),  \exists  y (P(\alpha)  \Rightarrow  ( \forall  x ( \forall  y P(y)))),  \exists  x ( \exists  y (P(x)  \Rightarrow  ( \forall  x ( \forall  y P(y)))))$\\
 from [4] by rule $ \Rightarrow \rightarrow $
\item $P(\alpha) \rightarrow   \forall  x ( \forall  y P(y)),  \exists  x ( \exists  y (P(x)  \Rightarrow  ( \forall  x ( \forall  y P(y))))),  \exists  y (P(\alpha)  \Rightarrow  ( \forall  x ( \forall  y P(y))))$\\
 from [5] by rule $\forall \rightarrow $ with new term $w1$
\item $P(\alpha) \rightarrow   \forall  y P(y),  \exists  y (P(\alpha)  \Rightarrow  ( \forall  x ( \forall  y P(y)))),  \exists  x ( \exists  y (P(x)  \Rightarrow  ( \forall  x ( \forall  y P(y)))))$\\
 from [6] by rule $\forall \rightarrow $ with new term $w2$
\item $P(\alpha) \rightarrow  P(w2),  \exists  x ( \exists  y (P(x)  \Rightarrow  ( \forall  x ( \forall  y P(y))))),  \exists  y (P(\alpha)  \Rightarrow  ( \forall  x ( \forall  y P(y))))$\\
 from [7] by rule $\exists \rightarrow $ with new term $\gamma$
\item $P(\alpha) \rightarrow  P(w2),  \exists  y (P(\alpha)  \Rightarrow  ( \forall  x ( \forall  y P(y)))),  \exists  x ( \exists  y (P(x)  \Rightarrow  ( \forall  x ( \forall  y P(y))))),  \exists  y (P(\gamma)  \Rightarrow  ( \forall  x ( \forall  y P(y))))$\\
  used in temporary unifications: [4]\\
 from [8] by rule $\exists \rightarrow $ with new term $\delta$
\item $P(\alpha) \rightarrow  P(w2), P(\alpha)  \Rightarrow  ( \forall  x ( \forall  y P(y))),  \exists  y (P(\gamma)  \Rightarrow  ( \forall  x ( \forall  y P(y)))),  \exists  x ( \exists  y (P(x)  \Rightarrow  ( \forall  x ( \forall  y P(y))))),  \exists  y (P(\alpha)  \Rightarrow  ( \forall  x ( \forall  y P(y))))$\\
  used in temporary unifications: [5]\\
 from [9] by rule $ \Rightarrow \rightarrow $
\item $P(\alpha) \rightarrow  P(w2),  \forall  x ( \forall  y P(y)),  \exists  y (P(\alpha)  \Rightarrow  ( \forall  x ( \forall  y P(y)))),  \exists  x ( \exists  y (P(x)  \Rightarrow  ( \forall  x ( \forall  y P(y))))),  \exists  y (P(\gamma)  \Rightarrow  ( \forall  x ( \forall  y P(y))))$\\
 from [10] by rule $\forall \rightarrow $ with new term $w3$
\item $P(\alpha) \rightarrow  P(w2),  \forall  y P(y),  \exists  y (P(\gamma)  \Rightarrow  ( \forall  x ( \forall  y P(y)))),  \exists  x ( \exists  y (P(x)  \Rightarrow  ( \forall  x ( \forall  y P(y))))),  \exists  y (P(\alpha)  \Rightarrow  ( \forall  x ( \forall  y P(y))))$\\
 from [11] by rule $\forall \rightarrow $ with new term $w4$
\item $P(\alpha) \rightarrow  P(w4), P(w2),  \exists  y (P(\alpha)  \Rightarrow  ( \forall  x ( \forall  y P(y)))),  \exists  x ( \exists  y (P(x)  \Rightarrow  ( \forall  x ( \forall  y P(y))))),  \exists  y (P(\gamma)  \Rightarrow  ( \forall  x ( \forall  y P(y))))$\\
 from [12] by rule $\exists \rightarrow $ with new term $\varepsilon$
\item $P(\alpha) \rightarrow  P(w2), P(w4), P(\gamma)  \Rightarrow  ( \forall  x ( \forall  y P(y))),  \exists  y (P(\gamma)  \Rightarrow  ( \forall  x ( \forall  y P(y)))),  \exists  x ( \exists  y (P(x)  \Rightarrow  ( \forall  x ( \forall  y P(y))))),  \exists  y (P(\alpha)  \Rightarrow  ( \forall  x ( \forall  y P(y))))$\\
  used in temporary unifications: [6]\\
 from [13] by rule $ \Rightarrow \rightarrow $
\item $P(\gamma), P(\alpha) \rightarrow  P(w4), P(w2),  \forall  x ( \forall  y P(y)),  \exists  y (P(\alpha)  \Rightarrow  ( \forall  x ( \forall  y P(y)))),  \exists  x ( \exists  y (P(x)  \Rightarrow  ( \forall  x ( \forall  y P(y))))),  \exists  y (P(\gamma)  \Rightarrow  ( \forall  x ( \forall  y P(y))))$\\
 from [14] by rule $\forall \rightarrow $ with new term $w5$
\item $P(\alpha), P(\gamma) \rightarrow  P(w2), P(w4),  \forall  y P(y),  \exists  y (P(\gamma)  \Rightarrow  ( \forall  x ( \forall  y P(y)))),  \exists  x ( \exists  y (P(x)  \Rightarrow  ( \forall  x ( \forall  y P(y))))),  \exists  y (P(\alpha)  \Rightarrow  ( \forall  x ( \forall  y P(y))))$\\
 from [15] by rule $\forall \rightarrow $ with new term $w6$
\item $P(\gamma), P(\alpha) \rightarrow  P(w6), P(w4), P(w2),  \exists  y (P(\alpha)  \Rightarrow  ( \forall  x ( \forall  y P(y)))),  \exists  x ( \exists  y (P(x)  \Rightarrow  ( \forall  x ( \forall  y P(y))))),  \exists  y (P(\gamma)  \Rightarrow  ( \forall  x ( \forall  y P(y))))$\\ 
 unification succeded using [$\gamma \mapsto w2$]
\end{enumerate}
%\end{document}
