\begin{enumerate}
\item $ \rightarrow  ( \forall  x (P(c1, x)  \vee  ( \forall  y P(x, y))))  \Rightarrow  ( \exists  x ( \forall  y P(x, y)))$\\
 from [2] by rule $ \Rightarrow \rightarrow $
\item $ \forall  x (P(c1, x)  \vee  ( \forall  y P(x, y))) \rightarrow   \exists  x ( \forall  y P(x, y))$\\
 from [3] by rule $\rightarrow \forall $ with new term $\alpha$
\item $P(c1, \alpha)  \vee  ( \forall  y P(\alpha, y)),  \forall  x (P(c1, x)  \vee  ( \forall  y P(x, y))) \rightarrow   \exists  x ( \forall  y P(x, y))$\\
 from [4] by rule $\exists \rightarrow $ with new term $\beta$
\item $P(c1, \alpha)  \vee  ( \forall  y P(\alpha, y)),  \forall  x (P(c1, x)  \vee  ( \forall  y P(x, y))) \rightarrow   \forall  y P(\beta, y),  \exists  x ( \forall  y P(x, y))$\\
 from [5] by rule $\forall \rightarrow $ with new term $w3$
\item $P(c1, \alpha)  \vee  ( \forall  y P(\alpha, y)),  \forall  x (P(c1, x)  \vee  ( \forall  y P(x, y))) \rightarrow  P(\beta, w3),  \exists  x ( \forall  y P(x, y))$\\
 from [6, 7] by rule $\rightarrow  \vee $
\item $P(c1, \alpha),  \forall  x (P(c1, x)  \vee  ( \forall  y P(x, y))) \rightarrow  P(\beta, w3),  \exists  x ( \forall  y P(x, y))$\\
  used in temporary unifications: [4]\\
 from [9] by rule $\rightarrow \forall $ with new term $\delta$
\item $ \forall  x (P(c1, x)  \vee  ( \forall  y P(x, y))),  \forall  y P(\alpha, y) \rightarrow  P(\beta, w3),  \exists  x ( \forall  y P(x, y))$\\
 from [8] by rule $\rightarrow \forall $ with new term $\gamma$
\item $P(\alpha, \gamma),  \forall  y P(\alpha, y),  \forall  x (P(c1, x)  \vee  ( \forall  y P(x, y))) \rightarrow  P(\beta, w3),  \exists  x ( \forall  y P(x, y))$\\
  used in temporary unifications: [6, 5, 4]\\
 from [12] by rule $\rightarrow \forall $ with new term $\zeta$
\item $P(c1, \alpha), P(c1, \delta)  \vee  ( \forall  y P(\delta, y)),  \forall  x (P(c1, x)  \vee  ( \forall  y P(x, y))) \rightarrow  P(\beta, w3),  \exists  x ( \forall  y P(x, y))$\\
  used in temporary unifications: [5]\\
 from [10] by rule $\exists \rightarrow $ with new term $\varepsilon$
\item $P(c1, \alpha), P(c1, \delta)  \vee  ( \forall  y P(\delta, y)),  \forall  x (P(c1, x)  \vee  ( \forall  y P(x, y))) \rightarrow  P(\beta, w3),  \forall  y P(\varepsilon, y),  \exists  x ( \forall  y P(x, y))$\\
  used in temporary unifications: [6]\\
 from [11] by rule $\forall \rightarrow $ with new term $w4$
\item $P(c1, \alpha), P(c1, \delta)  \vee  ( \forall  y P(\delta, y)),  \forall  x (P(c1, x)  \vee  ( \forall  y P(x, y))) \rightarrow  P(\varepsilon, w4), P(\beta, w3),  \exists  x ( \forall  y P(x, y))$\\
  used in temporary unifications: [7]\\ 
 unification succeded using [$\varepsilon \mapsto c1, \beta \mapsto \alpha, \alpha \mapsto w4$]
\item $P(\alpha, \zeta), P(\alpha, \gamma),  \forall  x (P(c1, x)  \vee  ( \forall  y P(x, y))),  \forall  y P(\alpha, y) \rightarrow  P(\beta, w3),  \exists  x ( \forall  y P(x, y))$\\
  used in temporary unifications: [7]\\ 
 unification succeded using [$\gamma \mapsto w3, \beta \mapsto \alpha, \alpha \mapsto w4$]
\end{enumerate}
