\begin{enumerate}
\item $ \rightarrow   \exists  x ( \exists  y (P(x)  \Rightarrow  ( \forall  x ( \forall  y P(y)))))$\\
 from [2] by rule $\exists \rightarrow $ with new term $\alpha$
\item $ \rightarrow   \exists  x ( \exists  y (P(x)  \Rightarrow  ( \forall  x ( \forall  y P(y))))),  \exists  y (P(\alpha)  \Rightarrow  ( \forall  x ( \forall  y P(y))))$\\
 from [3] by rule $\exists \rightarrow $ with new term $\beta$
\item $ \rightarrow  P(\alpha)  \Rightarrow  ( \forall  x ( \forall  y P(y))),  \exists  y (P(\alpha)  \Rightarrow  ( \forall  x ( \forall  y P(y)))),  \exists  x ( \exists  y (P(x)  \Rightarrow  ( \forall  x ( \forall  y P(y)))))$\\
 from [4] by rule $ \Rightarrow \rightarrow $
\item $P(\alpha) \rightarrow   \forall  x ( \forall  y P(y)),  \exists  x ( \exists  y (P(x)  \Rightarrow  ( \forall  x ( \forall  y P(y))))),  \exists  y (P(\alpha)  \Rightarrow  ( \forall  x ( \forall  y P(y))))$\\
 from [5] by rule $\forall \rightarrow $ with new term $w3$
\item $P(\alpha) \rightarrow   \forall  y P(y),  \exists  y (P(\alpha)  \Rightarrow  ( \forall  x ( \forall  y P(y)))),  \exists  x ( \exists  y (P(x)  \Rightarrow  ( \forall  x ( \forall  y P(y)))))$\\
 from [6] by rule $\forall \rightarrow $ with new term $w4$
\item $P(\alpha) \rightarrow  P(w4),  \exists  x ( \exists  y (P(x)  \Rightarrow  ( \forall  x ( \forall  y P(y))))),  \exists  y (P(\alpha)  \Rightarrow  ( \forall  x ( \forall  y P(y))))$\\ 
 unification succeded using [$\alpha \mapsto w4$]
\end{enumerate}
